proved adequacy of evaluation

ML_SP_Eval.v
@@ -7,12 +7,12 @@ Set Implicit Arguments.
 
 Require Import Arith List Metatheory.
 Require Import ML_SP_Definitions.
-Require Import ML_SP_Soundness.
+Require Import ML_SP_Rename.
 
 Module MkEval(Cstr:CstrIntf)(Const:CstIntf).
 
-Module Sound := MkSound(Cstr)(Const).
-Import Sound.
+Module Rename := MkRename(Cstr)(Const).
+Import Rename.Sound.
 Import Infra.
 Import Defs.
 Import Metatheory_Env.Env.
@@ -210,11 +210,136 @@ Definition trm2app t :=
   | _             => None
   end.
 
+Section Forall2.
+Variables A B : Set.
+Variable P : A -> B -> Prop.
+
+Inductive list_forall2 : list A -> list B -> Prop :=
+  | list_forall2_nil : list_forall2 nil nil
+  | list_forall2_cons : forall a b la lb,
+      P a b ->
+      list_forall2 la lb ->
+      list_forall2 (a::la) (b::lb).
+
+Hint Constructors list_forall2.
+
+Lemma list_forall2_sound : forall la lb,
+  list_forall2 la lb -> For_all2 P la lb.
+Proof.
+  induction 1; simpl*.
+Qed.
+
+Lemma list_forall2_complete : forall la lb,
+  For_all2 P la lb -> list_forall2 la lb.
+Proof.
+  induction la; intros; destruct lb; try contradiction; auto.
+  simpl in H; destruct* H.
+Qed.
+
+Lemma list_forall2_app : forall l1 l2 l3 l4,
+  list_forall2 l1 l3 -> list_forall2 l2 l4 ->
+  list_forall2 (l1 ++ l2) (l3 ++ l4).
+Proof.
+  intros until 1.
+  revert l2 l4.
+  induction H; simpl*.
+Qed.
+
+Lemma list_forall2_app_inv : forall l2 l4 l1 l3,
+  list_forall2 (l1 ++ l2) (l3 ++ l4) ->
+  length l1 = length l3 ->
+  list_forall2 l1 l3 /\ list_forall2 l2 l4.
+Proof.
+  induction l1; intros; destruct l3; try discriminate; simpl in *.
+    auto.
+  inversions H.
+  destruct* (IHl1 l3).
+Qed.
+
+Lemma list_forall2_length : forall l1 l2,
+  list_forall2 l1 l2 -> length l1 = length l2.
+Proof.
+  induction 1; simpl*.
+Qed.
+End Forall2.
+
+Hint Constructors list_forall2.
+Hint Resolve list_forall2_sound list_forall2_app list_forall2_length.
+Hint Immediate list_forall2_complete.
+
+Lemma clos_ok_nth : forall benv n0,
+  list_forall clos_ok benv ->
+  clos_ok (nth n0 benv clos_def).
+Proof.
+  intros.
+  destruct (le_lt_dec (length benv) n0).
+    rewrite* nth_overflow.
+  apply (list_forall_out H).
+  apply* nth_In.
+Qed.
+Hint Resolve clos_ok_nth.
+
+Inductive equiv_clos : clos -> clos -> Prop :=
+  | Equiv_clos_abs : forall t benv t' benv',
+      inst (trm_abs t) benv = inst (trm_abs t') benv' ->
+      equiv_clos (clos_abs t benv) (clos_abs t' benv')
+  | Equiv_clos_const : forall c args args',
+      list_forall2 equiv_clos args args' ->
+      equiv_clos (clos_const c args) (clos_const c args').
+Hint Constructors equiv_clos.
+
+Lemma equiv_cl : forall cl1 cl2,
+  equiv_clos cl1 cl2 -> clos2trm cl1 = clos2trm cl2.
+Proof.
+  induction cl1 using clos_ind'; intros; inversions H0; simpl*.
+  apply f_equal.
+  clear -H H4.
+  gen args'; induction H; intros; inversions H4; simpl*.
+  rewrite* (IHlist_forall lb).
+  rewrite* (H0 b).
+Qed.
+Hint Resolve equiv_cl.
+
+Lemma equiv_cls : forall cls1 cls2,
+  list_forall2 equiv_clos cls1 cls2 ->
+  List.map clos2trm cls1 = List.map clos2trm cls2.
+Proof.
+  induction 1; simpl; intros; auto*.
+  apply* f_equal2.
+Qed.
+
+Definition equiv_frame f1 f2 :=
+  inst (frm_trm f1) (frm_benv f1) = inst (frm_trm f2) (frm_benv f2) /\
+  list_forall2 equiv_clos (frm_app f1) (frm_app f2).
+
+Lemma list_forall2_refl : forall (A:Set) (P:A->A->Prop),
+  (forall x, P x x) ->
+  forall l, list_forall2 P l l.
+Proof.
+  induction l; simpl*.
+Qed.
+Hint Resolve list_forall2_refl.
+
+Lemma equiv_clos_refl : forall cl, equiv_clos cl cl.
+Proof.
+  induction cl using clos_ind'; constructor; auto.
+  induction H; auto.
+Qed.
+Hint Resolve equiv_clos_refl.
+
+Lemma equiv_cl_nth : forall n cls1 cls2,
+  list_forall2 equiv_clos cls1 cls2 ->
+  equiv_clos (nth n cls1 clos_def) (nth n cls2 clos_def).
+Proof.
+  intros; revert n; induction H; intros. simpl*.
+  destruct n; simpl*.
+Qed.
+
 Module Mk2(Delta:DeltaIntf).
 
-Module Sound2 := Sound.Mk2(Delta).
+Module Rename2 := Rename.Mk2(Delta).
+Import Rename2.
 Import Sound2.
-Import Sound.
 Import JudgInfra.
 Import Judge.
 
@@ -264,6 +389,11 @@ Module Type SndHypIntf2.
     reduce_clos c cls = (cl', cls') ->
     list_forall clos_ok cls ->
     list_forall clos_ok (cl' :: cls').
+  Parameter reduce_clos_ext : forall c args args',
+    list_forall2 equiv_clos args args' ->
+    let (cl,arg) := reduce_clos c args in
+    let (cl',arg') := reduce_clos c args' in
+    equiv_clos cl cl' /\ list_forall2 equiv_clos arg arg'.
   Parameter reduce_clos_sound :
     forall c cls (CLS : list_for_n clos_ok (S(Const.arity c)) cls) K E T,
       K; E |Gc|= const_app c (List.map clos2trm cls) ~: T ->
@@ -815,18 +945,6 @@ Proof.
   simpl.
   inversions* H2.
 Qed.
-
-Lemma clos_ok_nth : forall benv n0,
-  list_forall clos_ok benv ->
-  clos_ok (nth n0 benv clos_def).
-Proof.
-  intros.
-  destruct (le_lt_dec (length benv) n0).
-    rewrite* nth_overflow.
-  apply (list_forall_out H).
-  apply* nth_In.
-Qed.
-Hint Resolve clos_ok_nth.
 
 Lemma clos_ok_trm : forall benv K t T,
   list_forall clos_ok benv ->
@@ -1443,74 +1561,6 @@ Proof.
   rewrite* fold_left_app.
 Qed.
 
-Lemma eval_const : forall benv c t tl args,
-  inst t benv = const_app c tl ->
-  value (inst t benv) ->
-  list_forall value tl ->
-  exists cls1, exists cls2, exists t1, exists h,
-    trm2clos benv fenv t1 = clos_const c cls1 /\ trm_fv t1 = {} /\
-    eval fenv h benv args t nil = Inter (Frame benv (cls2 ++ args) t1 :: nil)
-    /\ List.map clos2trm (cls1 ++ cls2) = tl.
-Proof.
-  introv HI Val Htl.
-  gen_eq (inst t benv) as t'.
-  gen args t tl.
-  destruct Val as [n Val].
-  induction Val; simpl; intros.
-      puts (is_const_app c tl).
-      rewrite <- HI in H1; discriminate.
-    destruct t; try discriminate.
-      destruct (inst_clos2trm _ _ H); try discriminate.
-      case_rewrite R1 (nth n benv clos_def).
-      rewrite H0 in HI.
-      simpl in HI.
-      destruct (const_app_eq _ _ _ _ HI); subst; clear HI.
-      simpl in H0.
-      destruct (const_app_inv c (List.map clos2trm l)).
-        rewrite H1 in *. inversions H0.
-        esplit; exists (@nil clos); exists (trm_bvar n); exists 0; split*.
-        split*. destruct* l. discriminate.
-      destruct H1 as [t1 [t2 eq]].
-      rewrite eq in H0; discriminate.
-    inversions H; clear H.
-    destruct (const_app_inv c tl).
-      rewrite H in HI; inversions HI.
-      exists (@nil clos); exists (@nil clos); esplit;
-        exists 0; split; try split*; simpl*.
-    destruct H as [t1 [t2 eq]].
-    rewrite eq in HI; discriminate.
-  clear IHVal2.
-  destruct t; try discriminate.
-    destruct (inst_clos2trm _ _ H); try discriminate.
-    case_rewrite R1 (nth n0 benv clos_def).
-    rewrite H0 in HI. simpl in HI.
-    destruct (const_app_eq _ _ _ _ HI). subst.
-    exists l; exists (@nil clos); exists (trm_bvar n0); exists 0; split*.
-    split. simpl*.
-    rewrite* <- app_nil_end.
-  assert (value t2) by (esplit; auto*).
-  unfold trm_inst in H; simpl in H. inversions H; clear H.
-  destruct (eval_value _ _ H0) as [h2 [cl2 [eq2 eq2']]].
-  induction tl using rev_ind; try discriminate.
-  clear IHtl.
-  unfold const_app in HI; rewrite fold_left_app in HI.
-  simpl in HI; inversions HI; clear HI.
-  destruct* (IHVal1 (cl2::args) t3 tl)
-    as [cls1 [cls2 [t1 [h1 [eq1 [fv1 [eq1' eq1'']]]]]]].
-  exists cls1. exists (cls2 ++ cl2 :: nil).
-  exists t1; exists (S h2 + h1).
-  split*.
-  split; simpl*.
-  rewrite <- eval_restart_ok'.
-  rewrite eq2. simpl.
-  rewrite app_ass.
-  split*.
-  rewrite <- app_ass.
-  rewrite map_app.
-  rewrite eq1''.
-  simpl. rewrite* eq2'.
-Qed.
-
 Lemma app_eq_inv : forall (A:Set) (l3 l4 l1 l2 : list A),
   length l1 = length l2 ->
   l1 ++ l3 = l2 ++ l4 ->
@@ -1550,96 +1600,6 @@ Proof.
 Qed.
 Hint Immediate closed_n_inst.
 
-Section Forall2.
-Variables A B : Set.
-Variable P : A -> B -> Prop.
-
-Inductive list_forall2 : list A -> list B -> Prop :=
-  | list_forall2_nil : list_forall2 nil nil
-  | list_forall2_cons : forall a b la lb,
-      P a b ->
-      list_forall2 la lb ->
-      list_forall2 (a::la) (b::lb).
-
-Hint Constructors list_forall2.
-
-Lemma list_forall2_sound : forall la lb,
-  list_forall2 la lb -> For_all2 P la lb.
-Proof.
-  induction 1; simpl*.
-Qed.
-
-Lemma list_forall2_complete : forall la lb,
-  For_all2 P la lb -> list_forall2 la lb.
-Proof.
-  induction la; intros; destruct lb; try contradiction; auto.
-  simpl in H; destruct* H.
-Qed.
-
-Lemma list_forall2_app : forall l1 l2 l3 l4,
-  list_forall2 l1 l3 -> list_forall2 l2 l4 ->
-  list_forall2 (l1 ++ l2) (l3 ++ l4).
-Proof.
-  intros until 1.
-  revert l2 l4.
-  induction H; simpl*.
-Qed.
-
-Lemma list_forall2_app_inv : forall l2 l4 l1 l3,
-  list_forall2 (l1 ++ l2) (l3 ++ l4) ->
-  length l1 = length l3 ->
-  list_forall2 l1 l3 /\ list_forall2 l2 l4.
-Proof.
-  induction l1; intros; destruct l3; try discriminate; simpl in *.
-    auto.
-  inversions H.
-  destruct* (IHl1 l3).
-Qed.
-
-Lemma list_forall2_length : forall l1 l2,
-  list_forall2 l1 l2 -> length l1 = length l2.
-Proof.
-  induction 1; simpl*.
-Qed.
-End Forall2.
-
-Hint Constructors list_forall2.
-Hint Resolve list_forall2_sound list_forall2_app list_forall2_length.
-Hint Immediate list_forall2_complete.
-
-Inductive equiv_clos : clos -> clos -> Prop :=
-  | Equiv_clos_abs : forall t benv t' benv',
-      inst (trm_abs t) benv = inst (trm_abs t') benv' ->
-      equiv_clos (clos_abs t benv) (clos_abs t' benv')
-  | Equiv_clos_const : forall c args args',
-      list_forall2 equiv_clos args args' ->
-      equiv_clos (clos_const c args) (clos_const c args').
-Hint Constructors equiv_clos.
-
-Lemma equiv_cl : forall cl1 cl2,
-  equiv_clos cl1 cl2 -> clos2trm cl1 = clos2trm cl2.
-Proof.
-  induction cl1 using clos_ind'; intros; inversions H0; simpl*.
-  apply f_equal.
-  clear -H H4.
-  gen args'; induction H; intros; inversions H4; simpl*.
-  rewrite* (IHlist_forall lb).
-  rewrite* (H0 b).
-Qed.
-Hint Resolve equiv_cl.
-
-Lemma equiv_cls : forall cls1 cls2,
-  list_forall2 equiv_clos cls1 cls2 ->
-  List.map clos2trm cls1 = List.map clos2trm cls2.
-Proof.
-  induction 1; simpl; intros; auto*.
-  apply* f_equal2.
-Qed.
-
-Definition equiv_frame f1 f2 :=
-  inst (frm_trm f1) (frm_benv f1) = inst (frm_trm f2) (frm_benv f2) /\
-  list_forall2 equiv_clos (frm_app f1) (frm_app f2).
-
 (*
 Lemma app2trm'_equiv : forall args args' t,
   list_forall2 equiv_clos args args' ->
@@ -1675,39 +1635,10 @@ Proof.
 Qed.
 *)
 
-Parameter reduce_clos_ext : forall c args args',
-  list_forall2 equiv_clos args args' ->
-  let (cl,arg) := SH.reduce_clos c args in
-  let (cl',arg') := SH.reduce_clos c args' in
-  equiv_clos cl cl' /\ list_forall2 equiv_clos arg arg'.
-
 Lemma const_app_app : forall c l l',
   const_app c (l++l') = fold_left trm_app l' (const_app c l).
 Proof.
   intros. unfold const_app. apply fold_left_app.
-Qed.
-
-Lemma list_forall2_refl : forall (A:Set) (P:A->A->Prop),
-  (forall x, P x x) ->
-  forall l, list_forall2 P l l.
-Proof.
-  induction l; simpl*.
-Qed.
-Hint Resolve list_forall2_refl.
-
-Lemma equiv_clos_refl : forall cl, equiv_clos cl cl.
-Proof.
-  induction cl using clos_ind'; constructor; auto.
-  induction H; auto.
-Qed.
-Hint Resolve equiv_clos_refl.
-
-Lemma equiv_cl_nth : forall n cls1 cls2,
-  list_forall2 equiv_clos cls1 cls2 ->
-  equiv_clos (nth n cls1 clos_def) (nth n cls2 clos_def).
-Proof.
-  intros; revert n; induction H; intros. simpl*.
-  destruct n; simpl*.
 Qed.
 
 (*
@@ -1782,20 +1713,27 @@ Inductive eval_spec : eval_res -> eval_res -> Prop :=
       trm2app t = Some (t1, t2) ->
       eval_spec (Inter (Frame benv args t :: fl))
         (Inter (Frame benv nil t2 :: Frame benv args t1 :: fl))
-  | Eval_clos : forall benv args t fl r,
-      trm2app t = None ->
-      eval_cont (trm2clos benv fenv t) fl r ->
-      eval_spec (Inter (Frame benv args t :: fl)) r
   | Eval_abs : forall benv args t t1 benv' cl fl,
+      trm2app t = None ->
       trm2clos benv fenv t = clos_abs t1 benv' ->
       eval_spec (Inter (Frame benv (cl::args) t :: fl))
         (Inter (Frame (cl::benv') args t1 :: fl))
+  | Eval_abs' : forall benv t t1 benv' fl r,
+      trm2app t = None ->
+      trm2clos benv fenv t = clos_abs t1 benv' ->
+      eval_cont (clos_abs t1 benv') fl r ->
+      eval_spec (Inter (Frame benv nil t :: fl)) r
   | Eval_const : forall benv args t c cls1 cls2 cls3 fl,
+      trm2app t = None ->
+      trm2clos benv fenv t = clos_const c cls1 ->
       cls1 ++ args = cls2 ++ cls3 ->
+      length cls1 <= Const.arity c ->
       length cls2 = S(Const.arity c) ->
       eval_spec (Inter (Frame benv args t :: fl))
         (Inter (reduce_clos c cls2 cls3 :: fl))
   | Eval_const' : forall benv args t c cls1 fl r,
+      trm2app t = None ->
+      trm2clos benv fenv t = clos_const c cls1 ->
       length (cls1 ++ args) <= Const.arity c ->
       eval_cont (clos_const c (cls1++args)) fl r ->
       eval_spec (Inter (Frame benv args t :: fl)) r
@@ -1805,20 +1743,27 @@ Inductive eval_spec : eval_res -> eval_res -> Prop :=
 
 Hint Constructors eval_cont eval_spec.
 
-Lemma eval_spec_ok : forall r, eval_spec r (eval_restart 1 nil r).
+Lemma eval_spec_ok : forall r,
+  result_ok r ->
+  eval_spec r (eval_restart 1 nil r).
 Proof.
-  intros.
-  destruct r; simpl.
+  induction 1; simpl.
     rewrite plus_comm; simpl*.
-  destruct l as [|[benv args t] fl]. auto.
+  induction H as [|fl f Hfl IH [benv args t Hbenv Hargs Ht]]. auto.
   rewrite <- app_nil_end.
   case_eq (trm2app t); introv R1.
     destruct* p.
+  poses Ht2 (trm2clos_regular Hbenv Ht).
   destruct args.
-    apply* Eval_clos.
+    case_rewrite R2 (trm2clos benv fenv t).
+      apply* Eval_abs'.
+      destruct* fl.
+      destruct* f0.
+    apply* Eval_const'; rewrite <- app_nil_end.
+      inversion* Ht2.
     destruct* fl.
-    destruct* f.
-  case_eq (trm2clos benv fenv t); introv R2.
+    destruct* f0.
+  case_rewrite R2 (trm2clos benv fenv t).
     auto.
   case_eq (length l + length (c::args)); introv R3.
     destruct l; discriminate.
@@ -1832,8 +1777,14 @@ Proof.
     destruct (cut_ok _ H R5).
     subst.
     replace (c1::l2++l3) with ((c1::l2)++l3) in R4 by reflexivity.
-    puts (Eval_const benv (c::args) t _ _ _ fl R4 (f_equal S H0)).
-    unfold reduce_clos in H1.
+    assert (length l <= Const.arity c0).
+      clear IH.
+      assert (clos_ok (clos_const c0 l)).
+        rewrite <- R2.
+        destruct t; try discriminate; simpl*.
+      inversions* H1.
+    puts (Eval_const benv (c::args) t _ _ fl R1 R2 R4 H1 (f_equal S H0)).
+    unfold reduce_clos in H2.
     case_rewrite R6 (SH.reduce_clos c0 (c1::l2)).
     destruct* c2.
   apply* Eval_const'.
@@ -1841,7 +1792,60 @@ Proof.
     rewrite <- R3 in l0.
     rewrite* app_length.
   destruct* fl.
-  destruct* f.
+  destruct* f0.
+Qed.
+
+Lemma eval_spec_ok' : forall r r',
+  eval_spec r r' ->
+  r' = eval_restart 1 nil r.
+Proof.
+  induction 1; simpl; try rewrite H; try rewrite H0;
+    repeat rewrite <- app_nil_end; auto.
+  (* clos *)
+  inversions* H1.
+  (* const *)
+  puts (f_equal (@length _) H1).
+  do 2 rewrite app_length in H4.
+  destruct args.
+    rewrite <- app_nil_end in H1.
+    elimtype False.
+    simpl in H4; omega.
+  case_eq (length cls1 + length (c0::args)); introv R1.
+    destruct cls1; discriminate.
+  simpl in *.
+  destruct (le_lt_dec (Const.arity c) n); try solve [elimtype False; omega].
+  simpl.
+  rewrite H1.
+  destruct cls2. discriminate.
+  simpl.
+  simpl in H3. inversions H3; clear H3.
+  case_eq (cut (length cls2) (cls2 ++ cls3)); introv R2.
+  assert (length cls2 <= length (cls2 ++ cls3)).
+    rewrite app_length; omega.
+  destruct (cut_ok _ H3 R2).
+  assert (l0 = cls2 /\ l1 = cls3).
+    clear -H5 H7; gen l0.
+    induction cls2; destruct l0; simpl; intros; try discriminate. auto.
+    inversions H7.
+    destruct* (IHcls2 l0).
+    split; congruence.
+  destruct H8; subst.
+  unfold reduce_clos.
+  destruct (SH.reduce_clos c (c1 :: cls2)).
+  destruct* c2.
+  (* const' *)
+  destruct args.
+    rewrite <- app_nil_end in *.
+    inversions* H2.
+  case_eq (length cls1 + length (c0::args)); introv R1.
+    destruct cls1; discriminate.
+  destruct (le_lt_dec (Const.arity c) n); simpl.
+    elimtype False.
+    rewrite <- app_length in R1.
+    omega.
+  inversions* H2.
+  (* stop *)
+  apply f_equal2; auto; omega.
 Qed.
 
 Inductive equiv_result : eval_res -> eval_res -> Prop :=
@@ -1880,181 +1884,97 @@ Proof.
 Qed.
 Hint Immediate clos2trm_equiv.
 
+Lemma map_clos2trm_equiv : forall l1 l2,
+  List.map clos2trm l1 = List.map clos2trm l2 ->
+  list_forall2 equiv_clos l1 l2.
+Proof.
+  induction l1; destruct l2; simpl; intros; try discriminate; auto.
+  inversions* H.
+Qed.
+Hint Resolve map_clos2trm_equiv.
+
 Hint Extern 1 (equiv_result _ _) => solve [constructor; simpl; auto].
 Hint Extern 1 (list_forall2 _ _ _) => solve [constructor; simpl; auto].
 Hint Extern 1 (equiv_clos _ _) => solve [constructor; simpl; auto].
 Hint Extern 1 (equiv_frame _ _) => solve [constructor; simpl; auto].
 
-(*
-Lemma eval_bisim_app : forall t tl t' benv benv' args args' la lb,
-  inst (fold_left trm_app tl t) benv = inst t' benv' ->
-  list_forall2 equiv_clos args args' ->
-  list_forall2 equiv_frame la lb ->
-  list_forall frame_ok la ->
-  list_forall frame_ok lb ->
-  list_forall clos_ok benv ->
-  list_forall clos_ok args ->
-  list_forall (closed_n (length benv)) (t::tl) ->
-  list_forall clos_ok benv' ->
-  list_forall clos_ok args' ->
-  closed_n (length benv') t' ->
-  exists h1, exists h2,
-    equiv_result
-      (eval_restart h1 nil (Inter (Frame benv args (trm_bvar n) :: la)))
-      (eval_restart (h2+1) nil (Inter (Frame benv' args' t' :: lb))).
-Proof.
-  introv Eqt Eqargs Eqfl Hfl Hfl'.
-  intros Hbenv Hargs Ht Hbenv' Hargs' Ht'.
-*)
-
 Definition eq2 := eq.
 
-Lemma eval_bisim_bvar : forall n t' benv benv' args args' la lb,
-  inst (trm_bvar n) benv = inst t' benv' ->
-  list_forall2 equiv_clos args args' ->
-  list_forall2 equiv_frame la lb ->
-  list_forall frame_ok la ->
-  list_forall frame_ok lb ->
-  list_forall clos_ok benv ->
-  list_forall clos_ok args ->
-  closed_n (length benv) (trm_bvar n) ->
-  list_forall clos_ok benv' ->
-  list_forall clos_ok args' ->
-  closed_n (length benv') t' ->
-  exists h1, exists h2,
-    equiv_result
-      (eval_restart (h1+1) nil (Inter (Frame benv args (trm_bvar n) :: la)))
-      (eval_restart (h2+1) nil (Inter (Frame benv' args' t' :: lb))).
+Definition eval_res_cont r :=
+  match r with
+  | Result (S _) _ => true
+  | _ => false
+  end.
+
+Lemma equiv_result_restart0 : forall fl fl' r r',
+  equiv_result r r' ->
+  list_forall2 equiv_frame fl fl' ->
+  eval_res_cont r = false ->
+  equiv_result (eval_restart 0 fl r) (eval_restart 0 fl' r').
 Proof.
-  introv Eqt Eqargs Eqfl Hfl Hfl'.
-  intros Hbenv Hargs Ht Hbenv' Hargs' Ht'.
-  destruct (inst_clos2trm _ _ (sym_equal Eqt)).
-    case_rewrite R1 (nth n benv clos_def); simpl in H.
-      poses Hn (clos_ok_nth n Hbenv); rewrite R1 in Hn.
-      destruct t'; try discriminate.
-        destruct (inst_clos2trm _ _ (sym_equal H)); try discriminate.
-        case_rewrite R2 (nth n0 benv' clos_def).
-          poses Hn0 (clos_ok_nth n0 Hbenv'); rewrite R2 in Hn0.
-          exists 0; exists 0.
-          simpl.
-          rewrite R1; rewrite R2.
-          inversions Eqargs; clear Eqargs.
-            do 2 rewrite <- app_nil_end.
-            inversions *Eqfl; clear Eqfl.
-            destruct a; destruct b.
-            simpl.
-            destruct H1. simpl in H1, H3.
-            constructor; simpl.
-            inversions Hfl; inversions Hfl'; clear Hfl Hfl'.
-            inversions H7; inversions* H9.
-          remember (a::l) as benv1.
-          remember (b::l0) as benv2.
-          simpl in *.
-          inversions Hargs; inversions Hargs'; clear Hargs Hargs'.
-          inversions Hn.
-          repeat rewrite <- app_nil_end.
-          inversions* Hn0.
-        simpl in H0.
-        puts (is_const_app c (List.map clos2trm l0)).
-        rewrite <- H0 in H1; discriminate.
-      inversions H.
-      exists 0; exists 0; simpl.
-      rewrite R1.
-      repeat rewrite <- app_nil_end.
-      inversions Eqargs; clear Eqargs.
-        inversions* Eqfl; clear Eqfl.
-        destruct a; destruct b; simpl.
-        inversions H0; clear H0.
-        simpl in *. auto.
-      inversions Hn.
-      inversions* Ht'.
-    simpl.
-    repeat rewrite <- app_nil_end.
-    puts (clos_ok_nth n Hbenv).
-    rewrite R1 in H0.
-    destruct (eval_const _ _ _ args' H)
-      as [cls1 [cls2 [t1 [h [Eq1 [Fv1 [Eq' Eql]]]]]]].
-        rewrite* H.
-        apply (clos_ok_value H0).
-      inversions H0.
-      apply* list_forall_map.
-    exists 0; exists h.
-    do 2 rewrite <- eval_restart_ok'.
-    rewrite Eq'.
-    simpl.
-    rewrite R1; rewrite Eq1.
-    assert (equiv_clos (clos_const c (l++args))
-                    (clos_const c (cls1 ++ cls2 ++ args'))).
-      constructor.
-      rewrite <- app_ass.
-      apply* list_forall2_app.
-      clear -Eql.
-      gen l; induction (cls1++cls2) as [|cl cls]; intros;
-             destruct l; try discriminate; auto.
-      simpl in Eql; inversions Eql.
-      use (sym_equal H0).
-    case_eq (trm2app t1); introv R2.
-      destruct t1; try discriminate.
-    case_eq (cls2 ++ args'); introv R3.
-      inversions Eqargs; clear Eqargs; try (destruct cls2; discriminate).
-      repeat rewrite <- app_nil_end in *.
-      inversions* Eqfl; clear Eqfl; rewrite <- app_nil_end in H1; auto.
-      destruct a; destruct b; destruct H2; simpl in *; auto.
-    case_eq (length cls1 + length (c0 :: l0)); introv R4.
-      destruct cls1; discriminate.
-    inversions Eqargs; clear Eqargs.
-      repeat rewrite <- app_nil_end in *.
-      destruct (le_lt_dec (Const.arity c) n0); simpl.
-        elimtype False.
-        inversions H0.
-        rewrite <- app_length in R4.
-        puts (f_equal (@length _) Eql).
-        repeat rewrite map_length in H2.
-        omega.
-      inversions* Eqfl; clear Eqfl.
-      destruct a; destruct b; destruct H2; simpl in *; auto.
-    case_eq (length l + length (a :: la0)); introv R5.
-      destruct l; discriminate.
-    assert (n1 = n0).
-      rewrite <- R3 in R4.
-      rewrite app_length in R4.
-      puts (f_equal (@length _) Eql).
-      autorewrite with list in H4. simpl in *.
-      assert (length la0 = length lb0).
-      clear -H3; induction H3; simpl*.
-      omega.
-    subst.
-    destruct (le_lt_dec (Const.arity c) n0); simpl.
-      case_eq (l ++ a :: la0); introv R6. destruct l; discriminate.
-      case_eq (cls1 ++ c0 :: l0); introv R7. destruct cls1; discriminate.
-      case_eq (cut (Const.arity c) l2); introv R8.
-      case_eq (cut (Const.arity c) l3); introv R9.
-      assert (Const.arity c <= length l2).
-        puts (f_equal (@length _) R6).
-        rewrite app_length in H4. simpl in *; omega.
-      assert (Const.arity c <= length l3).
-        puts (f_equal (@length _) R7).
-        rewrite app_length in H5. simpl in *; omega.
-      destruct (cut_ok _ H4 R8).
-      destruct (cut_ok _ H5 R9).
-      subst.
-      assert (list_forall2 equiv_clos (c1 :: l4 ++ l5) (c2 :: l6 ++ l7)).
-        rewrite <- R7; rewrite <- R6.
-        rewrite <- R3.
-        inversions* H1.
-      inversions H7; clear H7.
-      destruct (list_forall2_app_inv _ _ _ _ H14). congruence.
-      puts (reduce_clos_ext c (list_forall2_cons _ _ H12 H7)).
-      destruct (SH.reduce_clos c (c1::l4)).
-      destruct (SH.reduce_clos c (c2::l6)).
-      destruct H10.
-      inversions* H10.
-    rewrite <- R3.
-    inversions* Eqfl; clear Eqfl.
-    destruct a0; destruct b0; destruct H4.
-    simpl in *; auto.
-  assert (term (trm_bvar n)). rewrite* <- H.
-  inversion H0.
+  induction 1; intros.
+    destruct n; try discriminate.
+    destruct H0; simpl*.
+    destruct a; destruct b; destruct H0; simpl in *; simpl*.
+  destruct H; simpl*.
+  destruct a; destruct b; destruct H0; simpl in *; simpl*.
+Qed.
+
+Lemma eval_const : forall benv c tl t args,
+  list_forall value tl ->
+  inst t benv = const_app c tl ->
+  exists cls1, exists cls2, exists t1, exists h,
+    trm2clos benv fenv t1 = clos_const c cls1 /\ trm_fv t1 = {} /\
+    eval fenv h benv args t nil = Inter (Frame benv (cls2 ++ args) t1 :: nil)
+    /\ List.map clos2trm (cls1 ++ cls2) = tl.
+Proof.
+  induction tl using rev_ind; introv Htl HI.
+    exists (@nil clos); exists (@nil clos).
+    destruct t; try discriminate.
+      destruct (inst_clos2trm _ _ (sym_equal HI)); try discriminate.
+      case_rewrite R1 (nth n benv clos_def).
+      simpl in H.
+      destruct (const_app_eq _ _ _ _ H); subst; clear H.
+      destruct l; try discriminate.
+      exists (trm_bvar n). exists 0.
+      split*.
+    inversions HI; clear HI.
+    exists (trm_cst c); exists 0.
+    split*.
+  rewrite const_app_app in HI.
+  destruct t; try discriminate.
+    clear IHtl.
+    destruct (inst_clos2trm _ _ (sym_equal HI)); try discriminate.
+    case_rewrite R1 (nth n benv clos_def).
+    rewrite <- const_app_app in H.
+    simpl in H.
+    destruct (const_app_eq _ _ _ _ H); subst; clear H.
+    exists l; exists (@nil clos).
+    exists (trm_bvar n); exists 0.
+    split*. split*. split*.
+    clear -H1.
+    rename l into cls1. rewrite <- app_nil_end. gen cls1.
+    induction (tl++x::nil); intros; destruct cls1; try discriminate.
+    auto.
+    simpl in H1; inversions* H1.
+  inversions HI.
+  assert (value (trm_inst_rec 0 (List.map clos2trm benv) t2))
+    by apply* (list_forall_out Htl).
+  destruct (eval_value _ _ H) as [h2 [cl2 [eq2a eq2']]].
+  destruct* (IHtl t1 (cl2::args))
+    as [cls1 [cls2 [t1' [h1 [eq1 [fv1 [eq1' eq1'']]]]]]].
+  exists cls1. exists (cls2 ++ cl2 :: nil).
+  exists t1'; exists (S h2 + h1).
+  split*.
+  split*.
+  simpl.
+  rewrite <- eval_restart_ok'.
+  rewrite eq2a. simpl.
+  rewrite app_ass.
+  split*.
+  rewrite <- app_ass.
+  rewrite map_app. simpl.
+  rewrite eq1''; rewrite* eq2'.
 Qed.
 
 Lemma equiv_clos_sym : forall cl1 cl2,
@@ -2104,30 +2024,172 @@ Proof.
   exists h2; exists* h1.
 Qed.
 
-Lemma eval_bisim : forall h0 args benv t fl args' benv' t' fl',
-  list_forall clos_ok args ->
-  list_forall clos_ok benv ->
-  closed_n (length benv) t ->
-  list_forall frame_ok fl ->
-  list_forall clos_ok args' ->
-  list_forall clos_ok benv' ->
-  closed_n (length benv') t' ->
-  list_forall frame_ok fl' ->
+Lemma eval_bisim_bvar : forall n t' benv benv' args args' la lb,
+  inst (trm_bvar n) benv = inst t' benv' ->
   list_forall2 equiv_clos args args' ->
-  inst t benv = inst t' benv' ->
-  list_forall2 equiv_frame fl fl' ->
-  exists h, exists h', h0 <= h /\ h0 <= h' /\
-    equiv_result (eval fenv h benv args t fl) (eval fenv h' benv' args' t' fl').
+  list_forall2 equiv_frame la lb ->
+  list_forall frame_ok la ->
+  list_forall frame_ok lb ->
+  list_forall clos_ok benv ->
+  list_forall clos_ok args ->
+  closed_n (length benv) (trm_bvar n) ->
+  list_forall clos_ok benv' ->
+  list_forall clos_ok args' ->
+  closed_n (length benv') t' ->
+  exists h1, exists h2,
+    equiv_result
+      (eval_restart (h1+1) nil (Inter (Frame benv args (trm_bvar n) :: la)))
+      (eval_restart (h2+1) nil (Inter (Frame benv' args' t' :: lb))).
 Proof.
-  induction h0; intros.
+  introv Eqt Eqargs Eqfl Hfl Hfl'.
+  intros Hbenv Hargs Ht Hbenv' Hargs' Ht'.
+  destruct (inst_clos2trm _ _ (sym_equal Eqt)).
+    case_rewrite R1 (nth n benv clos_def); simpl in H.
+      poses Hn (clos_ok_nth n Hbenv); rewrite R1 in Hn.
+      destruct t'; try discriminate.
+        destruct (inst_clos2trm _ _ (sym_equal H)); try discriminate.
+        case_rewrite R2 (nth n0 benv' clos_def).
+          poses Hn0 (clos_ok_nth n0 Hbenv'); rewrite R2 in Hn0.
+          exists 0; exists 0.
+          simpl.
+          rewrite R1; rewrite R2.
+          inversions Eqargs; clear Eqargs.
+            do 2 rewrite <- app_nil_end.
+            inversions *Eqfl; clear Eqfl.
+            destruct a; destruct b; destruct H1; simpl in *.
+            inversions Hfl; inversions Hfl'; clear Hfl Hfl'.
+            inversions H7; inversions* H9.
+          remember (a::l) as benv1.
+          remember (b::l0) as benv2.
+          simpl in *.
+          inversions Hargs; inversions Hargs'; clear Hargs Hargs'.
+          inversions Hn.
+          repeat rewrite <- app_nil_end.
+          inversions* Hn0.
+        simpl in H0.
+        puts (is_const_app c (List.map clos2trm l0)).
+        rewrite <- H0 in H1; discriminate.
+      inversions H.
+      exists 0; exists 0; simpl.
+      rewrite R1.
+      repeat rewrite <- app_nil_end.
+      inversions Eqargs; clear Eqargs.
+        inversions* Eqfl; clear Eqfl.
+        destruct a; destruct b; simpl.
+        inversions H0; clear H0.
+        simpl in *. auto.
+      inversions Hn.
+      inversions* Ht'.
+    simpl.
+    repeat rewrite <- app_nil_end.
+    puts (clos_ok_nth n Hbenv).
+    rewrite R1 in H0.
+    inversions H0.
+    assert (list_forall value (List.map clos2trm l)) by apply* list_forall_map.
+    destruct (eval_const _ _ _ args' H1 H)
+      as [cls1 [cls2 [t1 [h [Eq1 [Fv1 [Eq' Eql]]]]]]].
+    assert (equiv_clos (clos_const c (l++args))
+                    (clos_const c (cls1 ++ cls2 ++ args'))).
+      constructor.
+      rewrite <- app_ass.
+      apply* list_forall2_app.
+    clear H1.
+    exists 0; exists h.
+    do 2 rewrite <- eval_restart_ok'.
+    rewrite Eq'.
+    simpl.
+    rewrite R1; rewrite Eq1.
+    case_eq (trm2app t1); introv R2.
+      destruct t1; try discriminate.
+    case_eq (cls2 ++ args'); introv R3.
+      inversions Eqargs; clear Eqargs; try (destruct cls2; discriminate).
+      repeat rewrite <- app_nil_end in *.
+      inversions* Eqfl; clear Eqfl; rewrite <- app_nil_end in H2; auto.
+      destruct a; destruct b; destruct H1; simpl in *; auto.
+    case_eq (length cls1 + length (c0 :: l0)); introv R4.
+      destruct cls1; discriminate.
+    inversions Eqargs; clear Eqargs.
+      repeat rewrite <- app_nil_end in *.
+      destruct (le_lt_dec (Const.arity c) n0); simpl.
+        elimtype False.
+        inversions H0.
+        rewrite <- app_length in R4.
+        puts (f_equal (@length _) Eql).
+        repeat rewrite map_length in *.
+        omega.
+      inversions* Eqfl; clear Eqfl.
+      destruct a; destruct b; destruct H1; simpl in *; auto.
+    case_eq (length l + length (a :: la0)); introv R5.
+      destruct l; discriminate.
+    assert (n1 = n0).
+      rewrite <- R3 in R4.
+      rewrite app_length in R4.
+      puts (f_equal (@length _) Eql).
+      autorewrite with list in *. simpl in *.
+      puts (list_forall2_length H5).
+      omega.
+    subst.
+    destruct (le_lt_dec (Const.arity c) n0); simpl.
+      case_eq (l ++ a :: la0); introv R6. destruct l; discriminate.
+      case_eq (cls1 ++ c0 :: l0); introv R7. destruct cls1; discriminate.
+      case_eq (cut (Const.arity c) l2); introv R8.
+      case_eq (cut (Const.arity c) l3); introv R9.
+      assert (Const.arity c <= length l2).
+        puts (f_equal (@length _) R6).
+        rewrite app_length in H6. simpl in *; omega.
+      assert (Const.arity c <= length l3).
+        puts (f_equal (@length _) R7).
+        rewrite app_length in H7. simpl in *; omega.
+      destruct (cut_ok _ H6 R8).
+      destruct (cut_ok _ H7 R9).
+      subst.
+      assert (list_forall2 equiv_clos (c1 :: l4 ++ l5) (c2 :: l6 ++ l7)).
+        rewrite <- R7; rewrite <- R6.
+        rewrite <- R3.
+        inversions* H2.
+      inversions H9; clear H9.
+      destruct (list_forall2_app_inv _ _ _ _ H16). congruence.
+      puts (SH.reduce_clos_ext c (list_forall2_cons _ _ H14 H9)).
+      destruct (SH.reduce_clos c (c1::l4)).
+      destruct (SH.reduce_clos c (c2::l6)).
+      destruct H12.
+      inversions* H12.
+    rewrite <- R3.
+    inversions* Eqfl; clear Eqfl.
+    destruct a0; destruct b0; destruct H6.
+    simpl in *; auto.
+  assert (term (trm_bvar n)). rewrite* <- H.
+  inversion H0.
+Qed.
+
+Lemma eval_bisim : forall h0 r r',
+  equiv_result r r' ->
+  result_ok r ->
+  result_ok r' ->
+  exists h, exists h', h0 <= h /\ h0 <= h' /\
+    equiv_result (eval_restart h nil r) (eval_restart h' nil r').
+Proof.
+  introv Eqr Hr Hr'.
+  inversions Eqr; clear Eqr.
+    exists h0; exists h0; intuition.
+  inversions H; clear H.
+    exists h0; exists h0; intuition.
+  gen a b la lb; induction h0; intros.
     exists 0; exists 0; split*; split*.
-    simpl*.
-  destruct* (IHh0 args benv t fl args' benv' t' fl')
-    as [h [h' [Hh [Hh' Eqr]]]].
-  poses Hr (eval_regular h H H0 H1 H2).
-  poses Hr' (eval_regular h' H3 H4 H5 H6).
-  case_rewrite R1 (eval fenv h benv args t fl);
-    case_rewrite R2 (eval fenv h' benv' args' t' fl');
+    unfold eval_restart; simpl.
+    destruct a; destruct b; destruct H0.
+    simpl in *. auto.
+  destruct* (IHh0 _ _ H0 _ Hr _ H1 Hr') as [h [h' [Hh [Hh' Eqr]]]]; clear IHh0.
+  destruct a as [benv args t]; destruct b as [benv' args' t'].
+  destruct H0 as [Eqt Eqargs]. simpl in *.
+  repeat rewrite <- app_nil_end in *.
+  inversions Hr; inversions Hr'; clear Hr Hr'.
+  inversions H0; inversions H2; clear H2 H0.
+  inversions H5; inversions H7; clear H5 H7.
+  poses Hr (eval_regular h H8 H3 H9 H4).
+  poses Hr' (eval_regular h' H11 H10 H12 H6).
+  case_rewrite R1 (eval fenv h benv args t la);
+    case_rewrite R2 (eval fenv h' benv' args' t' lb);
     inversions Eqr; clear Eqr.
     exists (h+1); exists (h'+1). split. omega. split. omega.
     do 2 rewrite <- eval_restart_ok''.
@@ -2140,8 +2202,8 @@ Proof.
     exists (h + (h1+1)); exists (h'+(h2+1)). split. omega. split. omega.
     do 2 rewrite eval_restart_ok'' in Eqr.
     auto.
-  clear -fenv_ok Hr Hr' H12.
-  inversions H12; clear H12.
+  clear -fenv_ok Hr Hr' H2.
+  inversions H2; clear H2.
     exists 0; exists 0; simpl*.
   rename H0 into Eqfl.
   destruct a as [benv args t]; destruct b as [benv' args' t'].
@@ -2187,7 +2249,7 @@ Proof.
           inversions* H1.
         inversions H13; clear H13.
         destruct (list_forall2_app_inv _ _ _ _ H20). congruence.
-        puts (reduce_clos_ext c (list_forall2_cons _ _ H18 H13)).
+        puts (SH.reduce_clos_ext c (list_forall2_cons _ _ H18 H13)).
         destruct (SH.reduce_clos c (c0::l3)).
         destruct (SH.reduce_clos c (c1::l5)).
         destruct H16.
@@ -2220,13 +2282,332 @@ Proof.
     destruct (cut_ok _ l R4).
     subst.
     destruct (list_forall2_app_inv _ _ _ _ H0). congruence.
-    puts (reduce_clos_ext c0 (list_forall2_cons _ _ H H4)).
+    puts (SH.reduce_clos_ext c0 (list_forall2_cons _ _ H H4)).
     destruct (SH.reduce_clos c0 (a::l0)).
     destruct (SH.reduce_clos c0 (b::l2)).
     destruct H13.
     inversions* H13.
   inversions* Eqfl; clear Eqfl.
   destruct a0; destruct b0; destruct H1; simpl in *; auto.
+Qed.
+
+Lemma eval_abs : forall benv t' cls args t,
+  list_forall clos_ok cls ->
+  inst t benv = fold_left trm_app (List.map clos2trm cls) (trm_abs t') ->
+  exists l1, exists cls1, exists t1, exists h,
+    t = fold_left trm_app l1 t1 /\
+    list_forall2 (fun t cl => inst t benv = clos2trm cl) l1 cls1 /\
+    inst t1 benv = trm_abs t' /\
+    eval fenv h benv args t nil =
+    Inter (Frame benv (cls1 ++ args) t1 :: nil) /\
+    list_forall2 equiv_clos cls1 cls.
+Proof.
+  introv Hcls HI.
+  gen args t; induction cls using rev_ind; simpl; intros.
+    exists (@nil trm); exists (@nil clos); exists t; exists 0.
+    simpl. split*.
+  rewrite map_app in HI.
+  rewrite fold_left_app in HI.
+  destruct t; try discriminate.
+    elimtype False.
+    destruct (inst_clos2trm _ _ (sym_equal HI)); try discriminate.
+    destruct (nth n benv clos_def); try discriminate.
+    rewrite <- fold_left_app in H.
+    clear -H; simpl in H.
+    gen l; induction (List.map clos2trm cls ++ clos2trm x :: nil) using rev_ind;
+      intros.
+      puts (is_const_app c (List.map clos2trm l)).
+      rewrite <- H in H0; discriminate.
+    rewrite fold_left_app in H. simpl in H.
+    destruct l0 using rev_ind; try discriminate.
+    rewrite map_app in H; rewrite const_app_app in H.
+    inversions* H.
+  inversions HI.
+  assert (list_forall clos_ok cls) by auto.
+  assert (value (clos2trm x)) by auto.
+  rewrite <- H1 in H2.
+  destruct (eval_value _ _ H2) as [h' [cl' [He' Hx]]].
+  destruct (IHcls H (cl'::args) t1 H0)
+    as [l1 [cls1 [t3 [h [Ht [Hl1 [Ht' [He Eq]]]]]]]]; clear IHcls.
+  exists (l1 ++ t2 :: nil); exists (cls1 ++ cl'::nil); exists t3.
+  exists (h' + 1 + h).
+  intuition.
+      subst. rewrite* fold_left_app.
+    rewrite <- eval_restart_ok'.
+    rewrite app_ass. simpl app. rewrite <- He.
+    rewrite plus_comm. simpl.
+    replace h' with (h'+0) by omega. rewrite <- eval_restart_ok'.
+    rewrite He'.
+    simpl. auto.
+  apply* list_forall2_app.
+  constructor; auto.
+  apply clos2trm_equiv.
+  rewrite Hx.
+  rewrite <- H1.
+  auto.
+Qed.
+
+Hint Resolve list_forall_app.
+
+Hint Rewrite map_app fold_left_app : list.
+
+Lemma fold_app_eq_inv : forall t t' tl1 tl tl2,
+  fold_left trm_app tl t = fold_left trm_app (tl1 ++ tl2) t' ->
+  length tl = length tl2 ->
+  tl = tl2 /\ t = fold_left trm_app tl1 t'.
+Proof.
+  induction tl using rev_ind; intros; rewrite fold_left_app in *.
+    destruct tl2; try discriminate.
+    auto.
+  destruct tl2 using rev_ind.
+    rewrite app_length in H0; simpl in H0.
+    elimtype False; omega.
+  clear IHtl2.
+  autorewrite with list in *. simpl in *.
+  inversions H. rewrite <- fold_left_app in H2.
+  destruct* (IHtl tl2). omega.
+  subst*.
+Qed.
+
+Lemma fold_app_eq_inv' : forall t t' tl tl',
+  fold_left trm_app tl t = fold_left trm_app tl' t' ->
+  trm2app t = None -> trm2app t' = None ->
+  t = t' /\ tl = tl'.
+Proof.
+  induction tl using rev_ind; intros; destruct tl' using rev_ind; auto;
+    repeat rewrite fold_left_app in H; simpl in H; inversions H;
+    try discriminate.
+  clear IHtl'.
+  destruct* (IHtl tl'). subst*.
+Qed.
+
+Lemma inst_eq_equiv_clos : forall t benv t' benv',
+  trm2app t = None -> trm2app t' = None ->
+  closed_n (length benv) t -> closed_n (length benv') t' ->
+  inst t benv = inst t' benv' ->
+  equiv_clos (trm2clos benv fenv t) (trm2clos benv' fenv t').
+Proof.
+  intros.
+  destruct t; destruct t'; try discriminate;
+    try rewrite (inst_n _ H1) in *; try rewrite (inst_n _ H2) in *; auto.
+      destruct (nth n benv clos_def); try discriminate.
+      simpl in H3. 
+      puts (is_const_app c (List.map clos2trm l)).
+      rewrite H3 in H4; discriminate.
+    destruct (nth n benv' clos_def); try discriminate.
+    simpl in H3. 
+    puts (is_const_app c (List.map clos2trm l)).
+    rewrite <- H3 in H4; discriminate.
+  inversions* H3.
+Qed.
+
+Lemma eval_asym0 : forall benv args t fl benv' args' t' fl',
+  list_forall clos_ok args ->
+  list_forall clos_ok benv ->
+  list_forall frame_ok fl ->
+  list_forall clos_ok args' ->
+  list_forall clos_ok benv' ->
+  list_forall frame_ok fl' ->
+  closed_n (length benv) t ->
+  closed_n (length benv') t' ->
+  list_forall2 equiv_frame fl fl' ->
+  fold_left trm_app (List.map clos2trm args) (inst t benv) =
+  fold_left trm_app (List.map clos2trm args') (inst t' benv') ->
+  trm2app t = None ->
+  trm2app t' = None ->
+  length args <= length args' ->
+  equiv_result (eval fenv 1 benv args t fl) (eval fenv 1 benv' args' t' fl').
+Proof.
+  introv Hargs Hbenv Hfl. intros Hargs' Hbenv' Hfl' Ht Ht' Eqfl Eq R1 R2 l.
+  remember (cut (length args' - length args) args') as l'.
+  destruct l' as [args1' args2'].
+  forward~ (@cut_ok _ (length args' - length args) args' args1' args2').
+    omega.
+  intros [Hlen Eqargs]. subst. clear Heql'.
+  rewrite app_length in *.
+  assert (length args = length args2') by omega.
+  rewrite map_app in Eq.
+  destruct* (fold_app_eq_inv _ _ _ _ _ Eq) as [Eqargs Eqt].
+    repeat rewrite map_length; auto.
+  clear Eq Hlen.
+  replace 1 with (0+1+0) by omega.
+  do 4 rewrite <- eval_restart_ok'. simpl eval.
+  set (r := Inter (Frame benv args t :: nil)).
+  set (r' := Inter (Frame benv' (args1' ++ args2') t' :: nil)).
+  assert (Hr : result_ok r) by (unfold r; auto).
+  assert (Hr' : result_ok r') by (unfold r'; auto).
+  poses Er (eval_spec_ok Hr).
+  poses Er' (eval_spec_ok Hr').
+  set (e := eval_restart 1 nil r) in *; clearbody e.
+  set (e' := eval_restart 1 nil r') in *; clearbody e'.
+  subst r r'. clear Hr Hr'.
+  assert (equiv_result (eval_restart 0 fl e) (eval_restart 0 fl' e')
+          \/ exists c, exists l0, trm2clos benv fenv t = clos_const c l0
+             /\ exists l0', trm2clos benv' fenv t' = clos_const c l0'
+             /\ list_forall2 equiv_clos l0 (l0'++args1')).
+    destruct args1' using rev_ind.
+    simpl in Eqt.
+    puts (inst_eq_equiv_clos _ _ R1 R2 Ht Ht' Eqt).
+    inversions H0.
+        inversions Er; clear Er; try rewrite R1 in *;
+          try rewrite <- H1 in *; try discriminate;
+          inversions Er'; clear Er'; try rewrite R2 in *;
+            try rewrite <- H2 in *; try discriminate.
+          inversions H10; inversions H12; clear H9 H11 H10 H12.
+          simpl in * |- .
+          inversions Eqargs; clear Eqargs.
+          puts (trm2clos_regular Hbenv Ht). rewrite <- H1 in H4.
+          inversions H4; clear H4.
+          puts (trm2clos_regular Hbenv' Ht'). rewrite <- H2 in H4.
+          inversions H4; clear H4.
+          left; apply* equiv_result_restart0.
+        inversions H13; inversions H10; clear H10 H13 H9 H12.
+        inversions H14; inversions H11; clear H11 H14.
+        left; apply* equiv_result_restart0.
+      right; esplit; esplit; split*. esplit; split*.
+      rewrite* <- app_nil_end.
+    clear IHargs1'.
+    poses Eqt' Eqt.
+    autorewrite with list in Eqt'.
+    destruct t; try discriminate.
+    rewrite inst_n in *; auto. simpl.
+    destruct (nth n benv clos_def); try discriminate.
+    right; esplit; esplit; split*.
+    clear Eqt'.
+    simpl in Eqt; unfold const_app in Eqt.
+    destruct t'; try discriminate.
+          rewrite inst_n in Eqt; auto.
+          case_rewrite R3 (nth n0 benv' clos_def).
+            simpl in Eqt.
+            destruct* (fold_app_eq_inv' _ _ _ _ Eqt).
+            discriminate.
+          simpl in Eqt; unfold const_app in Eqt.
+          rewrite <- fold_left_app in Eqt.
+          destruct* (fold_app_eq_inv' _ _ _ _ Eqt).
+          inversions H0; clear H0.
+          exists l1.
+          rewrite <- map_app in H1; simpl*.
+        destruct* (fold_app_eq_inv' _ _ _ _ Eqt). discriminate.
+      destruct* (fold_app_eq_inv' _ _ _ _ Eqt). discriminate.
+    exists (@nil clos).
+    destruct* (fold_app_eq_inv' _ _ _ _ Eqt).
+    inversions H0. simpl*.
+  destruct* H0.
+  destruct H0 as [c [l0 [R4 [l0' [R5 Eql0']]]]].
+  assert (Eqcls:list_forall2 equiv_clos (l0 ++ args) (l0' ++ args1' ++ args2'))
+    by rewrite* <- app_ass.
+  poses Hlen (list_forall2_length Eqcls).
+  autorewrite with list in Hlen.
+  inversions Er; clear Er; rewrite R1 in *; try rewrite R4 in *;
+    try discriminate.
+    inversions H5; clear H4 H5.
+    inversions Er'; clear Er'; try rewrite R2 in *; try rewrite R5 in *;
+      try discriminate.
+      inversions H5; clear H5 H4.
+      rewrite H7 in Eqcls; rewrite H10 in Eqcls.
+      destruct (list_forall2_app_inv _ _ _ _ Eqcls). congruence.
+      unfold reduce_clos.
+      puts (SH.reduce_clos_ext c H0).
+      destruct (SH.reduce_clos c cls2).
+      destruct (SH.reduce_clos c cls4).
+      destruct H2.
+      inversions* H2.
+    inversions H6; clear H4 H6.
+    elimtype False.
+    puts (f_equal (@length _) H7).
+    autorewrite with list in *. simpl in *.
+    omega.
+  inversions H6; clear H6 H4.
+  inversions Er'; clear Er'; try rewrite R2 in *; try rewrite R5 in *;
+    try discriminate.
+    inversions H5; clear H5 H4.
+    puts (f_equal (@length _) H9).
+    autorewrite with list in *.
+    elimtype False; omega.
+  inversions H6; clear H4 H6.
+  inversions H8; clear H8.
+  inversions H10; clear H10.
+  apply* equiv_result_restart0.
+Qed.
+
+Lemma eval_asym : forall benv args t fl benv' args' t' fl',
+  list_forall clos_ok args ->
+  list_forall clos_ok benv ->
+  list_forall frame_ok fl ->
+  list_forall clos_ok args' ->
+  list_forall clos_ok benv' ->
+  list_forall frame_ok fl' ->
+  closed_n (length benv) t ->
+  closed_n (length benv') t' ->
+  list_forall2 equiv_frame fl fl' ->
+  fold_left trm_app (List.map clos2trm args) (inst t benv) =
+  fold_left trm_app (List.map clos2trm args') (inst t' benv') ->
+  trm2app t = None ->
+  trm2app t' = None ->
+  equiv_result (eval fenv 1 benv args t fl) (eval fenv 1 benv' args' t' fl').
+Proof.
+  intros.
+  destruct (le_lt_dec (length args) (length args')).
+    apply* eval_asym0.
+  apply equiv_result_sym.
+  apply* eval_asym0. omega.
+Qed.
+
+Lemma eval_args_eq : forall c l x args benv n fl,
+  list_forall clos_ok args ->
+  list_forall clos_ok benv ->
+  closed_n (length benv) (trm_bvar n) ->
+  nth n benv clos_def = clos_const c (l ++ x :: nil) ->
+  eval fenv 1 (clos_const c l :: nil) (x :: args) (trm_bvar 0) fl =
+  eval fenv 1 benv args (trm_bvar n) fl.
+Proof.
+  introv Hargs Hbenv Ht R1.
+  replace 1 with (0+1+0) by reflexivity.
+  do 4 rewrite <- eval_restart_ok'.
+  apply f_equal.
+  simpl eval.
+  set (benv2 := clos_const c l :: nil) in *.
+  poses Hn (clos_ok_nth n Hbenv).
+  rewrite R1 in Hn; inversions Hn.
+  rewrite app_length in H2; simpl in H2.
+  assert (Hbenv2: list_forall clos_ok benv2)
+    by (repeat (constructor; auto); omega).
+  set (r := Inter (Frame benv2 (x :: args) (trm_bvar 0) :: nil)).
+  set (r' := Inter (Frame benv args (trm_bvar n) :: nil)).
+  assert (result_ok r) by repeat (constructor; auto).
+  assert (result_ok r') by repeat (constructor; auto).
+  poses Er (eval_spec_ok H).
+  poses Er' (eval_spec_ok H0).
+  set (e := eval_restart 1 nil r) in *; clearbody e.
+  set (e' := eval_restart 1 nil r') in *; clearbody e'.
+  clear -Er Er' Hn R1.
+  subst r r' benv2.
+  replace (nth n benv clos_def) with (trm2clos benv fenv (trm_bvar n))
+    in R1 by reflexivity.
+  inversions Er; clear Er; try discriminate.
+  simpl in H4. inversions H4; clear H3 H4.
+    inversions Er'; clear Er'; try rewrite R1 in *; try discriminate.
+      inversions H4; clear H4 H3.
+      rewrite app_ass in H9.
+      simpl in H9; rewrite H6 in H9.
+      rewrite <- H11 in H8.
+      destruct (app_eq_inv _ _ _ _ H8 H9).
+      simpl.
+      subst*.
+    inversions H5; clear H3 H5.
+    elimtype False.
+    rewrite app_ass in H9; simpl in H9; rewrite H6 in H9.
+    rewrite app_length in H9; omega.
+  simpl in H5; inversions H5; clear H3 H5.
+  inversions H7; clear H7.
+  inversions Er'; clear Er'; try rewrite R1 in *; try discriminate.
+    inversions H4; clear H3 H4.
+    elimtype False.
+    rewrite app_ass in H7; simpl in H7; rewrite H7 in H6.
+    rewrite app_length in H6; omega.
+  inversions H5; clear H5.
+  inversions H8.
+  rewrite* app_ass.
 Qed.
 
 Lemma eval_complete_rec : forall args benv t fl args' benv' t' fl' K T,
@@ -2345,30 +2726,28 @@ Proof.
        rewrite app_length in Hlen. simpl in *; omega.
      rewrite H3 in H0.
      destruct (eval_value _ _ H0) as [h1 [cl1 [eq1 eq1']]].
-     destruct* (eval_const _ _ _ (cl4::args) (sym_equal H3) H0)
+     assert (Htl': list_forall value tl) by auto.
+     destruct* (eval_const _ _ _ (cl4::args) Htl' (sym_equal H3))
        as [cls1 [cls2 [t1' [h2 [Eq1 [Vt1' [Eq1' Eq1'']]]]]]].
      assert (E1: eval fenv (S h4 + h2) benv args (trm_app t1 t2) nil =
               Inter (Frame benv (cls2 ++ cl4 :: args) t1' :: nil)).
        simpl. rewrite <- eval_restart_ok'. rewrite* eq4.
-     remember (eval fenv ((S h4 + h2)+1) benv args (trm_app t1 t2) fl) as e.
-     poses E' Heqe.
-     (* exists ((S h4 + h2)+S h). *)
-     rewrite <- eval_restart_ok' in E'. rewrite E1 in E'.
-     simpl in E'.
-     case_rewrite R1 (trm2app t1').
-       destruct t1'; try discriminate.
-     case_rewrite R2 (cls2 ++ cl4 :: args).
-       destruct cls2; discriminate.
-     rewrite Eq1 in E'.
-     rewrite <- R2 in E'; simpl in E'.
-     case_rewrite R3 (cls1 ++ cls2 ++ cl4 :: args).
-       destruct cls1; destruct cls2; discriminate.
-     puts (f_equal (@length clos) R3).
-     rewrite app_length in H2; rewrite H2 in E'; clear H2. simpl in E'.
-     destruct (le_lt_dec (Const.arity c) (length l0)).
-       simpl in E'.
-       case_rewrite R4 (cut (Const.arity c) l0).
-       case_rewrite R5 (SH.reduce_clos c (c1 :: l2)).
+     assert (result_ok (Inter (Frame benv (cls2 ++ cl4 :: args) t1' :: nil))).
+       rewrite <- Eq1'.
+       assert (result_ok (Result 0 cl4)).
+         rewrite <- eq4. apply* eval_regular.
+         apply* closed_n_inst. 
+       inversions H2.
+       apply* eval_regular.
+       apply* closed_n_inst.
+     puts (eval_spec_ok H2).
+     rewrite <- Eq1' in H4 at 2.
+     assert (trm2app t1' = None) by (destruct* t1'; discriminate).
+     inversions H4; try rewrite H5 in *; try rewrite Eq1 in *; try discriminate.
+       inversion H12; clear H11 H12.
+       subst c0 cls0.
+       rewrite Eq1' in H10. rewrite <- E1 in H10.
+       clear Eq1' E1.
        destruct (typing_stack2trm_inv _ _ Typ) as [T' [K' Typ']].
          apply* is_bvar_term.
          apply* term_app2trm.
@@ -2377,152 +2756,98 @@ Proof.
          apply value_regular.
          rewrite* H3.
        destruct (typing_app2trm_inv _ _ Typ') as [T'' Typ''].
-         unfold const_app. rewrite fold_left_app. auto.
-       destruct (cut_ok _ l1 R4). subst l0.
-       assert (length (cls1 ++ cls2 ++ cl4 :: nil) = length (c1::l2)).
-         clear -H2 Hlen Eq1''.
-         rewrite <- app_ass.
-         rewrite app_length; simpl.
-         rewrite <- (map_length clos2trm).
-         rewrite Eq1''.
-         rewrite H2.
-         rewrite app_length in Hlen.
-         rewrite* Hlen.
-       destruct* (app_eq_inv args l3 _ _ H4).
-         repeat rewrite app_ass. simpl*.
-       subst l3.
-       rewrite <- H5 in R5.
-       assert (CLS: list_for_n clos_ok (S(Const.arity c))
-                      (cls1 ++ cls2 ++ cl4::nil)).
-         rewrite <- H2; split*.
-         clear Typ Typ''.
-         assert (closed_n (length benv) (trm_app t1 t2)) by auto.
-         puts (eval_regular (S h4 + h2) Hargs Hbenv H6
-                  (@list_forall_nil _ frame_ok)).
-         rewrite E1 in H7. rewrite <- R2 in *.
-         clear -Eq1 H7 fenv_ok.
-         inversions H7; clear H7.
+         rewrite const_app_app. auto.
+       assert (Hcls3: cls3 = cls1 ++ cls2 ++ cl4 :: nil /\ cls4 = args).
+         replace (cl4::args) with ((cl4::nil)++args) in H13.
+         rewrite Hlen in H15.
+         clear -H13 H15.
+         repeat rewrite <- app_ass in *.
+         assert (length cls3 = length ((cls1 ++ cls2) ++ cl4 :: nil)).
+           rewrite H15; autorewrite with list. simpl*.
+         apply* app_eq_inv.
+         simpl*.
+       destruct Hcls3 as [Hcls3]. subst cls4.
+       assert (CLS: list_for_n clos_ok (S(Const.arity c)) cls3).
+         clear Typ Typ' Typ''.
+         split*.
+         rewrite Hcls3.
+         clear -Eq1 H2 fenv_ok Hbenv.
+         inversions H2; clear H2.
          inversions H0; clear H0.
          inversions H3; clear H3.
          assert (clos_ok (clos_const c cls1)).
-           rewrite <- Eq1.
-           destruct t1'; try discriminate; simpl.
-               apply* clos_ok_nth.
-             case_eq (get v fenv); intros; auto.
-             apply (proj1 fenv_ok _ _ (binds_in H)).
-           constructor. auto. simpl; omega.
-         inversions* H.
-         apply list_forall_in; intros.
-         destruct (in_app_or _ _ _ H0). apply* (list_forall_out H3).
-         destruct (in_app_or _ _ _ H1); apply* (list_forall_out H5).
+           destruct t1'; try discriminate; simpl in Eq1.
+               rewrite* <- Eq1.
+             case_rewrite R1 (get v fenv).
+             subst. apply* (proj1 fenv_ok).
+           inversions* Eq1.
+         inversions H.
+         repeat (apply list_forall_app; auto).
        forward~ (SH.reduce_clos_sound CLS).
-         rewrite <- app_ass. rewrite map_app. rewrite Eq1''.
-         simpl. rewrite eq4'.
-         apply Typ''.
-       rewrite R5.
+         rewrite Hcls3.
+         rewrite <- app_ass.
+         rewrite map_app.
+         simpl.
+         rewrite* eq4'.
+       unfold reduce_clos in *.
+       destruct (SH.reduce_clos c cls3).
        generalize (list_for_n_value CLS).
+       rewrite Hcls3.
        rewrite <- app_ass.
-       rewrite map_app. rewrite Eq1''.
-       simpl List.map. rewrite eq4'.
+       rewrite map_app.
+       simpl.
+       rewrite eq4'.
        intros Hcls [Ok5 [Ok4 Eqred]].
        rewrite (ProofIrrelevance.proof_irrelevance _ vl Hcls) in H.
-       puts (trans_equal Eqred H); clear H Eqred Typ Typ' Typ''.
-       destruct c2.
-         clear -Eqargs Eqfl Ok5 Ok4 H6 Hbenv' Ht' Heqe E'.
-         poses E2 (f_equal (eval_restart 1 nil) E').
-         simpl in E2. rewrite <- app_nil_end in E2.
-         remember (eval fenv 0 benv' args' t' fl') as e'.
-         poses E3 Heqe'. simpl in E3.
-         gen args args' t'; induction l4 using rev_ind; intros.
-           destruct t'; try discriminate.
-             simpl in E3.
-             exists h. subst; simpl.
-             destruct (inst_clos2trm _ _ H6); try discriminate.
-             inversions Eqargs; clear Eqargs.
-               inversions* Eqfl; clear Eqfl.
-               destruct a; destruct b; destruct H0; simpl in *; auto.
-             case_rewrite R1 (nth n benv' clos_def).
-               inversions H.
-               repeat (constructor; simpl*).
-               inversions Ok5.
-               puts (clos_ok_nth n Hbenv').
-               rewrite R1 in H2.
-               inversions* H2.
-             elimtype False.
-             puts (is_const_app c (List.map clos2trm l)).
-             simpl in H; rewrite <- H in H2; discriminate.
-           exists h; subst. simpl.
-           inversions Eqargs; clear Eqargs.
-             inversions* Eqfl; clear Eqfl.
-             destruct a; destruct b; destruct H; simpl in *; auto.
-           repeat (constructor; simpl*).
-           inversions Ok5.
-           inversions* Ht'.
-         rewrite map_app in H6; rewrite fold_left_app in H6; simpl in H6.
-         destruct t'; try discriminate.
-           clear IHl4. elimtype False.
-           destruct (inst_clos2trm _ _ H6); try discriminate.
-           case_rewrite R1 (nth n benv' clos_def).
-           simpl in H. unfold const_app in H.
-           induction l using rev_ind. discriminate.
-           rewrite map_app in H; rewrite fold_left_app in H.
-           inversions H. clear -H1.
-           gen l4; induction l using rev_ind; destruct l4 using rev_ind;
-             repeat (rewrite map_app; rewrite fold_left_app);
-             simpl; intros; try discriminate.
-           inversions H1; clear H1.
-           elim (IHl _ H0).
-         inversions H6.
-         assert (clos_ok x) by auto.
-         assert (list_forall clos_ok l4) by auto.
-         clear Ok4.
-         puts (clos_ok_value H). rewrite H1 in H3.
-         destruct (eval_value _ _ H3) as [h1 [cl [eq1 eq2]]].
-         puts (clos2trm_equiv _ _ (trans_equal H1 (sym_equal eq2))).
-         inversions Ht'.
-         destruct* (IHl4 H2 _ _ (list_forall2_cons _ _ H4 Eqargs) t'1).
-         exists (S h + x0). rewrite <-eval_restart_ok'.
-         remember 1 as h.
-         simpl.
-         replace x0 with (x0+0) by omega.
-         rewrite <- eval_restart_ok'.
-         
-         inversions Eqargs; clear Eqargs.
-           inversions* Eqfl; clear Eqfl.
-               destruct a; destruct b; destruct H0; simpl in *; auto.
-             case_rewrite R1 (nth n benv' clos_def).
-             inversions H.
-             repeat (constructor; simpl*).
-             inversions Ok5.
-             puts (clos_ok_nth n Hbenv').
-             rewrite R1 in H2.
-             inversions* H2.
-       inversions H6; clear H6.
-       destruct (IHl4 (x::args) 
-         
-           simpl.
-         assert (exists h', 
-         simpl in H6.
-         subst h.
-
- repeat (constructor; simpl; auto).
-           rewrite <- H. refine (trans_equal _ Eqred). simpl.
-       unfold trm_inst in Eqred.
-       rewrite <- Eqred.
-       destruct c2; simpl.
-         unfold app2trm'. rewrite map_app. rewrite* fold_left_app.
-       rewrite trm_inst_nil.
-       unfold app2trm'. do 2 rewrite map_app.
-       do 2 rewrite fold_left_app. auto.
-     elimtype False.
-     puts Hlen.
-     rewrite <- Eq1'' in H2.
-     rewrite app_length in H2.
-     rewrite map_length in H2; simpl in H2.
-     puts (f_equal (@length clos) R3).
-     rewrite <- app_ass in H4.
-     rewrite app_length in H4. simpl in H4.
-     omega.
+       puts (trans_equal Eqred H). clear H Eqred.
+       destruct c0.
+         simpl in H6. unfold trm_inst in H6. simpl in H6.
+         destruct (eval_abs benv' _ args' t' Ok4 (sym_equal H6))
+           as [l1 [cls4 [t4 [h4' [Ht4 [Hl1 [Ht4' [He4 Hcls4]]]]]]]].
+         exists (S h4 + h2 +1 +0); exists (h4'+0).
+         do 2 rewrite <- eval_restart_ok'. rewrite <- H10.
+         rewrite <- eval_restart_ok'. rewrite He4.
+         apply* equiv_result_restart0.
+       simpl in H6. rewrite <- const_app_app in H6. rewrite <- map_app in H6.
+       assert (list_forall value (List.map clos2trm (l0++l))).
+         rewrite map_app.
+         inversions Ok5.
+         apply list_forall_app; apply* list_forall_map.
+       destruct (eval_const benv' c0 _ args' H (sym_equal H6))
+           as [l1 [cls4 [t4 [h4' [Ht4 [Fvs4 [He4 Hcls4]]]]]]].
+       case_eq (trm2app t4); introv R1.
+         destruct t4; discriminate.
+       exists (S h4 + h2 +1 +1); exists (h4'+1).
+       do 2 rewrite <- eval_restart_ok'. rewrite <- H10.
+       rewrite <- eval_restart_ok'. rewrite He4.
+       unfold eval_restart. simpl app.
+       assert (result_ok (Inter (Frame benv' (cls4 ++ args') t4 :: nil))).
+         rewrite <- He4.
+         apply* eval_regular.
+       inversions H7; clear H7.
+       inversions H9; clear H9.
+       inversions H12; clear H11 H12.
+       apply* eval_asym.
+         inversions* Ok5.
+       rewrite <- app_ass.
+       rewrite map_app. 
+       rewrite <- Hcls4.
+       assert (List.map clos2trm args = List.map clos2trm args').
+         clear -Eqargs; induction* Eqargs. simpl.
+         rewrite (equiv_cl H). congruence.
+         rewrite H7.
+       repeat rewrite map_app.
+       destruct t4; try discriminate.
+           rewrite* inst_n. simpl in Ht4; rewrite Ht4.
+           simpl; unfold const_app. rewrite <- fold_left_app.
+           rewrite* app_ass.
+         assert (v \in {{v}}) by auto.
+         simpl in Fvs4. rewrite Fvs4 in H8. elim (in_empty H8).
+       autorewrite with list.
+       simpl in Ht4. inversions* Ht4.
+     inversions H12.
+     clear - Hlen H13.
+     autorewrite with list in *. simpl in *. elimtype False; omega.
     destruct t; try discriminate.
       destruct (inst_clos2trm _ _ H1).
         destruct (nth n benv clos_def). discriminate.
@@ -2542,21 +2867,23 @@ Proof.
         simpl in H1. puts (is_const_app c (List.map clos2trm l)).
         rewrite <- H1 in H2; discriminate.
       discriminate.
-    unfold trm_inst in H0; inversions H0; clear H0.
+    inversions H0; clear H0.
     assert (list_forall frame_ok (Frame benv args (trm_abs t4) :: fl)) by auto.
     assert (Ht'2: closed_n (S (length benv')) t'2).
       rewrite <- (map_length clos2trm).
-      apply (@closed_n_inst (List.map clos2trm benv') t'2 1).
+      apply (@closed_n_inst_rec (List.map clos2trm benv') t'2 1).
       rewrite <- H3.
       assert (clos_ok (clos_abs t4 benv)) by auto.
       puts (term_closed_0 (clos_ok_term H1)).
       simpl in H2. unfold trm_inst in H2. inversions* H2.
     assert (list_forall frame_ok (Frame benv' args' (trm_abs t'2) :: fl'))
       by auto.
-    forward~ (IHRed t3 t'1 nil (list_forall_nil clos_ok) benv' Hbenv' _ H1
-               _ (list_forall_nil clos_ok) I _ Hbenv H7 Eqbenv _ H0).
-       split*. split*. simpl. unfold equiv_trm, trm_inst; simpl. rewrite* H3.
-       simpl*. rewrite* (equiv_cls _ _ Eqbenv).
+    inversions Ht'.
+    forward~ (IHRed t3 t'1 nil (list_forall_nil clos_ok) benv' Hbenv' H10
+               _ H1 _ (list_forall_nil clos_ok) (@list_forall2_nil _ _ _) _
+               Hbenv H7 _ H0).
+       repeat (constructor; simpl; auto). 
+       unfold inst, trm_inst; simpl. apply* f_equal.
       simpl.
       rewrite* is_bvar_term.
     intros [h3 [h3' eq3]].
@@ -2568,226 +2895,239 @@ Proof.
      destruct (clos_ok_value (clos_ok_nth n Hbenv)).
      rewrite <- H2 in H.
      inversions H. esplit; auto*.
-    destruct (typing_stack2trm_inv _ _ Typ) as [T' [K' Typ']].
-      apply* is_bvar_term.
-    destruct (typing_app2trm_inv _ _ Typ') as [T'' Typ'']. auto.
-    inversions Typ''; try discriminate.
-    unfold trm_inst in H1; inversion H1; clear H1.
+   (*destruct (typing_stack2trm_inv _ _ Typ) as [T' [K' Typ']].
+     apply* is_bvar_term.
+   destruct (typing_app2trm_inv _ _ Typ') as [T'' Typ'']. auto.
+   inversions Typ''; try discriminate. *)
+   unfold trm_inst in H1; inversion H1; clear H1.
+   inversions Ht.
+   destruct (eval_value _ _ H) as [h4 [cl4 [Eq4 Eq4c]]].
+   assert (Hcl4: clos_ok cl4).
+     assert (result_ok (Result 0 cl4)).
+     rewrite <- Eq4.
+     apply* eval_regular.
+     inversions* H1.
+   assert (Hargs1: list_forall clos_ok (cl4::args)) by auto.
+   destruct t'; try discriminate.
+     destruct (inst_clos2trm _ _ H0); try discriminate.
+     puts (clos_ok_nth n Hbenv').
+     case_rewrite R1 (nth n benv' clos_def).
+     rewrite H0 in *.
+     simpl in H1.
+     rewrite <- H0 in H1.
+     destruct l using rev_ind. discriminate.
+     clear IHl.
+     rewrite map_app in H1; rewrite const_app_app in H1.
+     simpl in H1; inversions H1; clear H1.
+     assert (clos_ok x) by inversions* H2.
+     assert (Hargs2: list_forall clos_ok (x::args')) by auto.
+     assert (Eqargs1: list_forall2 equiv_clos (cl4::args) (x::args')).
+       constructor; auto.
+       apply clos2trm_equiv.
+       rewrite <- H5.
+       rewrite* Eq4c.
+     pose (benv2 := clos_const c l :: nil).
+     assert (Hbenv2: list_forall clos_ok benv2).
+       unfold benv2. inversions H2.
+       repeat constructor; auto.
+       rewrite app_length in H9; simpl in H9; omega.
+     assert (closed_n (length benv2) (trm_bvar 0)) by auto.
+     forward~ (IHRed t3 _ _ Hargs2 _ Hbenv2 H3 _ Hfl' _
+       Hargs1 Eqargs1 _ Hbenv H6 _ Hfl); clear IHRed.
+       eapply retypable_stack2trm; try apply Typ; auto.
+       unfold app2trm; simpl.
+       apply* retypable_app2trm.
+       rewrite Eq4c.
+       apply retypable_trm_app; auto.
+     intros [h3 [h3' eq3]].
+     destruct (eval_bisim 1 eq3) as [h2 [h2' [le [le' Eq2]]]].
+         apply* eval_regular.
+       apply* eval_regular.
+     destruct h2'. elimtype False; omega.
+     exists (1 + h4 + h3 + h2); exists (h3' + 1 + h2'). simpl.
+     do 2 rewrite <- eval_restart_ok'. rewrite Eq4. simpl.
+     do 2 rewrite <- eval_restart_ok''.
+     rewrite plus_comm.
+     rewrite <- eval_restart_ok'.
+     rewrite* <- (@eval_args_eq c l x).
+     rewrite eval_restart_ok'.
+     rewrite plus_comm.
+     rewrite (eval_restart_ok'' h2').
+     rewrite <- plus_assoc.
+     rewrite* <- eval_restart_ok''.
+   inversions H0.
+   rewrite H3 in H.
+   destruct (eval_value _ _ H) as [h2 [cl2 [Eq2 Eq2c]]].
+   assert (Hcl2: clos_ok cl2).
+     assert (result_ok (Result 0 cl2)).
+       rewrite <- Eq2.
+       apply* eval_regular.
+       inversions* Ht'.
+     inversions* H1.
+   assert (Hargs2: list_forall clos_ok (cl2::args')) by auto.
+   assert (Eqargs1: list_forall2 equiv_clos (cl4::args) (cl2::args')).
+     constructor; auto.
+     apply clos2trm_equiv.
+     rewrite Eq2c.
+     rewrite* Eq4c.
+   inversions Ht'.
+   forward~ (IHRed t3 t'1 _ Hargs2 _ Hbenv' H5 _ Hfl' _
+        Hargs1 Eqargs1 _ Hbenv H6 _ Hfl); clear IHRed.
+     eapply retypable_stack2trm; try apply Typ; auto.
+       apply* term_app2trm.
+       constructor; apply* term_inst_closed.
+     unfold app2trm; simpl.
+     apply* retypable_app2trm.
+     rewrite Eq4c.
+     apply retypable_trm_app; auto.
+   intros [h3 [h3' eq3]].
+   exists (1+h4+h3); exists (1+h2+h3'). simpl.
+   do 2 rewrite <- eval_restart_ok'. rewrite Eq4. rewrite Eq2. simpl.
+   auto.
+  destruct t; try discriminate.
+    destruct (inst_clos2trm _ _ H1); try discriminate.
+    elim (@value_irreducible t2 t2'); auto.
+    clear -H2 Hbenv.
+    destruct (clos_ok_value (clos_ok_nth n Hbenv)).
+    rewrite <- H2 in H.
+    inversions H. esplit; auto*.
+  unfold trm_inst in H1; inversion H1; clear H1.
+  destruct t'; try discriminate.
+    destruct (inst_clos2trm _ _ H0); try discriminate.
+    puts (clos_ok_nth n Hbenv').
+    case_rewrite R1 (nth n benv' clos_def).
+    rewrite H0 in *.
+    simpl in H1.
+    rewrite <- H0 in H1.
+    destruct l using rev_ind. discriminate.
+    clear IHl.
+    rewrite map_app in H1; rewrite const_app_app in H1.
+    simpl in H1; inversions H1; clear H1.
+    assert (clos_ok x) by inversions* H2.
+    pose (benv2 := x :: nil).
+    assert (Hbenv2: list_forall clos_ok benv2) by (unfold benv2; auto).
+    assert (closed_n 1 (trm_bvar 0)) by auto.
     inversions Ht.
-    destruct t'; try discriminate.
-      destruct (inst_clos2trm _ _ H0); try discriminate.
-      (*
-      puts (clos_ok_nth n Hbenv).
-      puts (clos_ok_value H2).
-      rewrite <- H1 in H3.
-      case_rewrite R1 (nth n benv clos_def).
-      rewrite H0 in *.
-      simpl in H1.
-      destruct (eval_const _ _ _ args H1 H3)
-        as [cls1 [cls2 [t1 [h [Eq1 [Fv1 [Eq2 Eq3]]]]]]].
-        inversions H2. apply* list_forall_map. intros; apply* clos_ok_value.
-      *)
-      puts (clos_ok_nth n Hbenv').
-      case_rewrite R1 (nth n benv' clos_def).
-      destruct l using rev_ind. discriminate. clear IHl.
-      destruct (eval_value _ _ H) as [h4 [cl4 [Eq4 Eq4c]]].
-      (* rewrite (trm_inst_equiv benv benv') in H.
-      destruct (eval_value _ _ H) as [h4' [cl4' [Eq4' Eq4c']]]. *)
-      simpl in H1; rewrite map_app in H1; rewrite const_app_app in H1.
-      simpl in H1; inversions H1; clear H1.
-      assert (Hcl4: clos_ok cl4).
-        assert (result_ok (Result 0 cl4)).
-        rewrite <- Eq4.
-        apply* eval_regular.
-        inversions* H1.
-      clear Typ' Typ''.
-      assert (list_forall clos_ok (cl4::args)) by auto.
-      assert (Hx: clos_ok x) by inversions* H2.
-      assert (list_forall clos_ok (x::args')) by auto.
-      assert (For_all2 equiv_clos (cl4::args) (x::args')).
-        simpl. split*. unfold equiv_clos. rewrite Eq4c. rewrite* <- H5.
-      forward~ (IHRed t3 (const_app c (List.map clos2trm l)) (x::args') H3
-        benv' Hbenv' _ Hfl' _ H1 H4 _ Hbenv H7 Eqbenv _ Hfl); clear IHRed.
-        eapply retypable_stack2trm; try apply Typ; auto.
-        unfold app2trm; simpl.
-        apply retypable_app2trm; auto.
-        rewrite Eq4c.
-        apply retypable_trm_app; auto.
-        symmetry; apply term_trm_inst.
-        puts (clos_ok_term H2).
-        simpl in H10; unfold const_app in H10.
-        rewrite map_app in H10; rewrite fold_left_app in H10; simpl in H10.
-        inversions* H10.
-      intros [h3 [h3' eq3]].
-      exists (Datatypes.S h4 + h3); exists h3'. simpl.
-      rewrite <- eval_restart_ok'. rewrite Eq4. simpl.
-      rewrite eq3.
-      assert (exists h', res2trm'
-        (eval fenv h3' benv' (x :: args') (const_app c (List.map clos2trm l))
-          fl') = res2trm' (eval fenv h' benv' args' (trm_bvar n) fl')).
-        set (l' := x :: nil) in *.
-        replace (x::args') with (l'++args') by reflexivity.
-        assert (const_app c (List.map clos2trm (l++l')) =
-                trm_inst (trm_bvar n) (List.map clos2trm benv')).
-          unfold l'; rewrite map_app; rewrite const_app_app; simpl.
-          rewrite* <- H5.
-        clearbody l'; clear - H2 R1 Eqbenv Hbenv' H10.
-        set (l'' := l') in R1.
-        assert (Eql: For_all2 equiv_clos l' l'').
-          unfold equiv_clos, equiv_trm, l''; clear; induction l'; simpl*.
-        clearbody l''.
-        gen h3' l' l''; induction l using rev_ind; intros.
-          unfold const_app.
-          simpl in *.
-          exists h3'.
-          destruct h3'. simpl.
-            rewrite <- H10.
-            unfold app2trm'; rewrite map_app; rewrite fold_left_app.
-            reflexivity.
-          simpl.
-          rewrite R1.
-          destruct l'; destruct l''; try contradiction.
-            destruct args'; simpl*.
-          simpl.
-          destruct (le_lt_dec (Const.arity c) (length (l'++args'))); simpl.
-            destruct args'.
-              elimtype False.
-              inversions H2. simpl in H3; rewrite <- app_nil_end in l.
-              omega.
-            rewrite app_length in l.
-            destruct (le_lt_dec (Const.arity c)(length l''+ length(c2::args')));
-              try solve [elimtype False; omega].
-            simpl.
-            case_eq (cut (Const.arity c) (l'++c2::args')); introv R2.
-            case_eq (cut (Const.arity c) (l''++c2::args')); introv R3.
-            rewrite <- app_length in l,l0.
-            destruct (cut_ok _ l R2).
-            destruct (cut_ok _ l0 R3).
-            assert (For_all2 equiv_clos (l1 ++ l2) (l3 ++ l4)).
-              rewrite <- H0. rewrite <- H3.
-              simpl in Eql; destruct Eql.
-              apply* For_all2_app.
-            destruct (For_all2_app_inv _ _ _ _ _ H4). congruence.
-            simpl in Eql; destruct Eql.
-            puts (reduce_clos_ext c (c0 :: l1) (c1 :: l3) (conj H7 H5)).
-            destruct (SH.reduce_clos c (c0 :: l1)).
-            destruct (SH.reduce_clos c (c1 :: l3)).
-            simpl in H9; destruct H9.
-            unfold equiv_clos in H9.
-            destruct c3. simpl in H9.
-              destruct c4; simpl in H9.
-                
-              
-  
-            reflexivity.
-          destruct args'.
-            rewrite <- app_nil_end. auto.
-          rewrite app_length in l.
-          destruct (le_lt_dec (Const.arity c) (length l'+ length(c1::args')));
-            try solve [elimtype False; omega].
-          simpl. reflexivity.
-        destruct h3'.
-          exists 0; simpl.
-          rewrite <- H10.
-          simpl.
-          unfold app2trm'; rewrite map_app.
-          rewrite fold_left_app.
-          unfold trm_inst; rewrite* term_trm_inst.
-            rewrite (map_app _ (l++x::nil)). rewrite* const_app_app.
-          puts (term_closed_0 (clos_ok_term H2)). simpl in H.
-          rewrite map_app in H.
-          rewrite const_app_app in H.
-          revert H; generalize (const_app c (List.map clos2trm (l++x::nil))).
-          generalize (List.map clos2trm l').
-          clear; intros; induction l using rev_ind. auto.
-          rewrite fold_left_app in H. simpl in H.
-          inversions* H.
-        rewrite app_ass in *. simpl in * |-.
-        rewrite map_app in *.
-        rewrite const_app_app in *.
-        simpl fold_left.
-        simpl.
-        inversions H2.
-        assert (Hx: clos_ok x) by auto.
-        destruct (eval_value benv' (clos2trm x)) as [h [cl [eq1 eq2]]].
-          unfold trm_inst.
-          rewrite* term_trm_inst.
-          apply* clos_ok_value.
-        destruct (le_lt_dec h h3').
-          replace h3' with (h + (h3'-h)) by omega.
-          rewrite <- eval_restart_ok'.
-          rewrite eq1.
-          simpl.
-          replace (cl::l'++args') with ((cl::l')++args') by reflexivity.
-          assert (clos_ok cl).
-            assert (result_ok (Result 0 cl)).
-              rewrite <- eq1.
-              apply* eval_regular.
-            inversions* H.
-          apply* IHl.
-            constructor; auto. clear -H H1.
-              apply list_forall_in; intros. destruct* (in_app_or _ _ _ H0).
-                apply* (list_forall_out H1).
-              simpl in H2; destruct H2. subst*.
-              apply* (list_forall_out H1).
-            rewrite app_length in *; simpl in *. auto.
-          
-
-
-        destruct IHh3' as [h' Eq].
-        exists (S h').
-        destruct l using rev_ind.
-          simpl in * |-. unfold const_app; simpl fold_left.
-          simpl.
-          SearchAbout term.
-        unfold app2trm'; simpl.
-        unfold trm_inst in Eq4c; rewrite <- Eq4c.
-        unfold trm_inst. rewrite* term_trm_inst .
-        
-      assert (
-      destruct h3'. simpl.
-        unfold trm_inst at 2.
-        rewrite* <- (trm_inst_equiv benv benv'); auto.
-        unfold trm_inst in H0; rewrite <- H0.
-        unfold app2trm'; simpl.
-        unfold trm_inst in Eq4c; rewrite <- Eq4c.
-        unfold trm_inst. rewrite* term_trm_inst .
-      simpl.
-        rewrite <- H0.
-      assert (list_forall frame_ok (Frame benv' args' (trm_abs t'2) :: fl'))
-      by auto.
-      
-      discriminate.
-    unfold trm_inst in H0; inversions H0; clear H0.
-    assert (list_forall frame_ok (Frame benv args (trm_abs t4) :: fl)) by auto.
-    assert (Ht'2: closed_n (S (length benv')) t'2).
-      rewrite <- (map_length clos2trm).
-      apply (@closed_n_inst (List.map clos2trm benv') t'2 1).
-      rewrite <- (equiv_cls _ _ Eqbenv).
-      rewrite <- H3.
-      assert (clos_ok (clos_abs t4 benv)) by auto.
-      puts (term_closed_0 (clos_ok_term H1)).
-      simpl in H2. unfold trm_inst in H2. inversions* H2.
-    assert (list_forall frame_ok (Frame benv' args' (trm_abs t'2) :: fl'))
-      by auto.
-    forward~ (IHRed t3 t'1 nil (list_forall_nil clos_ok) benv' Hbenv' _ H1
-               _ (list_forall_nil clos_ok) I _ Hbenv H7 Eqbenv _ H0).
-       split*. split*. simpl. unfold equiv_trm, trm_inst; simpl. rewrite* H3.
-       simpl*.
+    assert (Hfl1: list_forall frame_ok (Frame benv args t3 :: fl)) by auto.
+    assert (Hfl2: list_forall frame_ok
+           (Frame (clos_const c l :: nil) args' (trm_bvar 0) :: fl')).
+      inversions H2.
+      repeat constructor; auto.
+      rewrite app_length in H10; simpl in H10; omega.
+    forward~ (IHRed t4 _ _ (@list_forall_nil _ _)  _ Hbenv2 H3 _ Hfl2 _
+       (@list_forall_nil _ _) (list_forall2_nil equiv_clos) _ Hbenv H9 _ Hfl1);
+      clear IHRed.
       simpl.
       rewrite* is_bvar_term.
+      eapply retypable_stack2trm; try apply Typ; auto.
+      unfold app2trm; simpl.
+      apply* retypable_app2trm.
+      apply* retypable_trm_app.
     intros [h3 [h3' eq3]].
-    exists (S h3); exists (S h3'). simpl*.
-   
+    destruct (eval_bisim 2 eq3) as [h2 [h2' [le [le' Eq2]]]].
+        apply* eval_regular.
+      inversions H2.
+      apply eval_regular; repeat (constructor; auto).
+        rewrite app_length in H10; simpl in H10; omega.
+      auto.
+    destruct h2'. elimtype False; omega.
+    do 2 rewrite eval_restart_ok'' in Eq2.
+    replace (h3'+S h2') with (1+h3'+h2') in Eq2 by omega.
+    rewrite <- (eval_restart_ok'' h2') in Eq2.
+    simpl in Eq2.
+    rewrite eval_restart_ok'' in Eq2.
+    destruct h2'. elimtype False; omega.
+    exists (1+h3+h2). simpl. exists (1+(h3'+h2')).
+    rewrite <- (eval_restart_ok'' (h3'+h2')).
+    rewrite* <- (@eval_args_eq c l x).
+    rewrite (eval_restart_ok'' (h3'+h2')).
+    replace (1+(h3'+h2')) with (h3'+S h2') by omega.
+    auto.
+  inversions H0.
+  inversions Ht.
+  inversions Ht'.
+  assert (Hfl1: list_forall frame_ok (Frame benv args t3 :: fl)) by auto.
+  assert (Hfl2: list_forall frame_ok (Frame benv' args' t'1 :: fl')) by auto.
+  forward~ (IHRed t4 t'2 _ (@list_forall_nil _ _)  _ Hbenv' H8 _ Hfl2 _
+    (@list_forall_nil _ _) (list_forall2_nil equiv_clos) _ Hbenv H6 _ Hfl1);
+      clear IHRed.
+    simpl.
+    rewrite* is_bvar_term.
+    eapply retypable_stack2trm; try apply Typ; auto.
+    unfold app2trm; simpl.
+    apply* retypable_app2trm.
+    apply* retypable_trm_app.
+  intros [h3 [h3' eq3]].
+  exists (S h3). exists (S h3'). simpl*.
+Qed.
+
+Lemma eval_count_rev : forall cl n h fl,
+  result_ok (Inter fl) ->
+  eval_restart h nil (Inter fl) = Result n cl ->
+  eval_restart (h-n) nil (Inter fl) = Result 0 cl.
+Proof.
+  induction n; introv Hr H. rewrite <- minus_n_O. auto.
+  destruct h. simpl in H. destruct fl as [|[benv args t]]; discriminate.
+  replace (S h - S n) with (h - n) by omega.
+  apply IHn; clear IHn. auto.
+  replace (S h) with (h + 1) in H by omega.
+  unfold eval_restart in H.
+  destruct fl; try discriminate.
+  destruct f as [benv args t].
+  rewrite <- eval_restart_ok in H.
+  case_rewrite R1 (eval fenv h benv args t fl).
+    simpl in H. inversions H.
+    rewrite plus_comm in H1; inversions H1.
+    unfold eval_restart. rewrite* <- app_nil_end.
+  assert (result_ok (Inter l)).
+    inversions Hr. inversions H1. inversions H4.
+    rewrite <- R1; apply* eval_regular.
+  puts (eval_spec_ok H0).
+  rewrite H in H1.
+  inversions H1; clear H1.
+    inversions H5.
+  inversion H6.
+Qed.
 
 Theorem eval_complete : forall K t t' T,
   K ; E |Gc|= t ~: T ->
-  clos_refl_trans _ red t t' ->
+  clos_refl_trans_1n _ red t t' ->
   value t' ->
-  exists h,
-    eval fenv h nil nil t nil = Result c /\
-    untyped t' = untyped (clos2trm cl).
-
+  exists h, exists cl,
+    eval fenv h nil nil t nil = Result 0 cl /\
+    t' = clos2trm cl.
+Proof.
+  intros.
+  gen K; induction H0; intros.
+    rewrite <- trm_inst_nil in H1.
+    replace (@nil trm) with (List.map clos2trm nil) in H1 by auto.
+    destruct (eval_value _ _ H1) as [h [cl [Eq Hcl]]].
+    unfold inst in Hcl. simpl in Hcl. rewrite trm_inst_nil in Hcl.
+    esplit; esplit; split*.
+  puts (preservation_result (typing_gc_any H2) H).
+  destruct (typing_remove_gc H3 {} (F:=E)) as [K' [_ Typ]].
+      intro; intros. exists (@nil kind). rewrite* <- app_nil_end.
+    auto.
+  destruct (IHclos_refl_trans_1n H1 _ Typ) as [h [cl [Eq Hz]]].
+  forward~ (@eval_complete_rec nil nil x nil nil nil y nil K T).
+      unfold app2trm, inst; simpl. rewrite* trm_inst_nil.
+    unfold inst; simpl. do 2 rewrite trm_inst_nil. auto.
+  intros [h0 [h' Eq']].
+  destruct (eval_bisim (h-h') Eq') as [h1 [h2 [le1 [le2 Eq1]]]].
+      apply* eval_regular.
+    apply* eval_regular.
+  do 2 rewrite eval_restart_ok' in Eq1.
+  replace (h' + h2) with (h + (h2 + h' - h)) in Eq1 by omega.
+  rewrite <- (eval_restart_ok' (h2+h'-h)) in Eq1. rewrite Eq in Eq1.
+  simpl in Eq1.
+  inversions Eq1; clear Eq1.
+  assert (result_ok (Inter (Frame nil nil x :: nil))) by auto.
+  replace (h0 + h1) with (0+(h0+h1)) in H4 by omega.
+  rewrite <- eval_restart_ok' in H4. simpl eval in H4.
+  puts (eval_count_rev _ H5 (sym_equal H4)).
+  simpl in H7.
+  esplit; esplit; split*.
+Qed.
 
 End Soundness.
 
